Leansubst/Basic.lean
@@ -7,18 +7,20 @@ import Leansubst.Defs
 
 namespace Leansubst.Subst'
 
+section
+
 variable {σ : Type}
-variable (s t u : Subst σ)
-variable (i : Nat) (x : σ)
+variable (s t u : Subst' σ)
+variable (i j k : Nat) (x : σ)
 variable (e : Expr σ) (es : List (Expr σ))
 
-local notation:arg "⟦" a "⟧" => Quotient.mk _ a
+local notation:arg "⟦" a "⟧" => Quotient.mk (Subst'.setoid σ) a
 
 def up : Nat → Subst' σ → Subst' σ
   | 0,     s => s
   | i + 1, s => cons (.var 0) (comp (up i s) (shift 1))
 
-theorem get_up_low (i j k : Nat) (h : k < j) : (up j (@shift σ i)).get k = .var k := by
+theorem get_up_low (h : k < j) : (up j (@shift σ i)).get k = .var k := by
   induction j generalizing k with
   | zero => intros; contradiction
   | succ j ih =>
@@ -36,7 +38,7 @@ theorem get_up_low (i j k : Nat) (h : k < j) : (up j (@shift σ i)).get k = .var
         specialize ih _ (Nat.le_of_lt_succ h)
         rw [get, comp_def, ih, apply]
 
-theorem get_up_high (i j k : Nat) (h : j ≤ k) : (up j (@shift σ i)).get k = .var (k + i) := by
+theorem get_up_high (h : j ≤ k) : (up j (@shift σ i)).get k = .var (k + i) := by
   have ⟨d, hd⟩ := Nat.le.dest h; clear h
   induction j generalizing k d with
   | zero => rfl
@@ -49,7 +51,7 @@ theorem get_up_high (i j k : Nat) (h : j ≤ k) : (up j (@shift σ i)).get k = .
       rw [Nat.succ_add] at hd; injection hd with hd
       rw [ih _ _ hd, apply, Nat.succ_add]
 
-theorem comp_eqv_comps (i j : Nat) : comp (up j (shift i)) (shift 1) ≈ (comps (up j (shift i)) 1 : Subst' σ) := by
+theorem comp_eqv_comps_special : comp (up j (shift i)) (shift 1) ≈ (comps (up j (shift i)) 1 : Subst' σ) := by
   intros k
   rw [comp_def, comps_def]
   cases Nat.lt_sum_ge k j with
@@ -65,7 +67,7 @@ theorem comp_eqv_comps (i j : Nat) : comp (up j (shift i)) (shift 1) ≈ (comps 
     case inr h => exact (h (Nat.zero_le _)).elim
 
 /-- We have to show that `applys` actually agrees with `apply shift`. -/
-theorem applys_def (i j : Nat) : applys j i e = apply (up j (shift i)) e := by
+theorem applys_def : applys j i e = apply (up j (shift i)) e := by
   revert j
   -- Induction on `e`.
   apply @Expr.recOn _
@@ -94,7 +96,7 @@ theorem applys_def (i j : Nat) : applys j i e = apply (up j (shift i)) e := by
   case binder e ih j =>
     rw [applys, apply, ih, up]
     congr 1
-    have h := comp_eqv_comps i j (σ := σ)
+    have h := comp_eqv_comps_special i j (σ := σ)
     have h' : (.cons (.var 0) ⟦comp (up j (shift i)) (shift 1)⟧ : Subst σ) e =
               (.cons (.var 0) ⟦comps (up j (shift i)) 1⟧ : Subst σ) e := by rw [Quotient.sound h]
     exact h'
@@ -110,6 +112,14 @@ theorem applys_def (i j : Nat) : applys j i e = apply (up j (shift i)) e := by
         rw [applys, apply] at ih'
         injection ih'
 
+theorem apply_apply : t (s e) = (comp s t) e := by
+  sorry
+
+theorem id_apply : (id σ) e = e := by
+  sorry
+
+end
+
 end Subst'
 
 namespace Subst
@@ -123,25 +133,33 @@ namespace Subst
 @[simp] theorem comps_wrap (s : Subst' σ) (n : Nat) : ⟦Subst'.comps s n⟧ = Subst.comps ⟦s⟧ n := rfl
 @[simp] theorem comp_wrap (s t : Subst' σ) : ⟦Subst'.comp s t⟧ = Subst.comp ⟦s⟧ ⟦t⟧ := rfl
 
+section
+
 variable {σ : Type}
 variable (s t u : Subst σ)
-variable (i : Nat) (x : σ)
+variable (i j k : Nat) (x : σ)
 variable (e : Expr σ) (es : List (Expr σ))
+
+local notation:arg "⟦" a "⟧" => Quotient.mk (Subst'.setoid σ) a
 
 @[simp]
 theorem get_zero : (cons e s).get 0 = e := by
-  induction s using Quotient.inductionOn
+  induction s using Quotient.ind
   rw [← cons_wrap, ← get_wrap]
   rfl
 
 @[simp]
 theorem get_succ : (cons e s).get (i + 1) = s.get i := by
-  induction s using Quotient.inductionOn
+  induction s using Quotient.ind
   rw [← cons_wrap, ← get_wrap]
   rfl
 
 @[simp]
-theorem shift_expand : shift σ (i + 1 + 1) = comp (shift σ (i + 1)) (shift σ 1) := by
+theorem shift_zero : shift σ 0 = id σ := by
+  rfl
+
+@[simp]
+theorem shift_succ_succ : shift σ (i + 1 + 1) = comp (shift σ (i + 1)) (shift σ 1) := by
   simp only [← shift_wrap, ← comp_wrap]
   apply Quotient.sound
   intros j
@@ -149,7 +167,7 @@ theorem shift_expand : shift σ (i + 1 + 1) = comp (shift σ (i + 1)) (shift σ 
 
 @[simp]
 theorem comps_expand : comps s i = comp s (shift σ i) := by
-  induction s using Quotient.inductionOn
+  induction s using Quotient.ind
   rw [← comps_wrap, ← shift_wrap, ← comp_wrap]
   apply Quotient.sound
   intros j
@@ -158,18 +176,18 @@ theorem comps_expand : comps s i = comp s (shift σ i) := by
 
 @[simp]
 theorem apply_var : s (.var i) = s.get i := by
-  induction s using Quotient.inductionOn
+  induction s using Quotient.ind
   rw [← apply_wrap, ← get_wrap, Subst'.apply_var]
 
 @[simp]
 theorem apply_binder : s (.binder e) = .binder ((cons (.var 0) (comp s (shift σ 1))) e) := by
-  induction s using Quotient.inductionOn
+  induction s using Quotient.ind
   rw [← apply_wrap, Subst'.apply]
-  simp
+  simp only [apply_wrap, cons_wrap, comps_wrap, comps_expand]
 
 @[simp]
 theorem apply_node : s (.node x es) = .node x (es.map s) := by
-  induction s using Quotient.inductionOn
+  induction s using Quotient.ind
   induction es with
   | nil => rw [List.map, ← apply_wrap, Subst'.apply, Subst'.apply.nested]
   | cons h t ih =>
@@ -179,20 +197,20 @@ theorem apply_node : s (.node x es) = .node x (es.map s) := by
 
 @[simp]
 theorem apply_apply : t (s e) = (comp s t) e := by
-  induction s using Quotient.inductionOn; rename_i s
-  induction t using Quotient.inductionOn; rename_i t
+  induction s using Quotient.ind; rename_i s
+  induction t using Quotient.ind; rename_i t
   simp only [← comp_wrap, ← apply_wrap]
-  sorry
+  exact Subst'.apply_apply _ _ _
 
 @[simp]
 theorem id_apply : (id σ) e = e := by
   rw [← id_wrap, ← apply_wrap]
   rw [Subst'.id]
-  sorry
+  exact Subst'.id_apply _
 
 @[simp]
 theorem id_comp : comp (id σ) s = s := by
-  induction s using Quotient.inductionOn
+  induction s using Quotient.ind
   rw [← id_wrap, ← comp_wrap]
   apply Quotient.sound
   intros j
@@ -201,49 +219,51 @@ theorem id_comp : comp (id σ) s = s := by
 
 @[simp]
 theorem comp_id : comp s (id σ) = s := by
-  induction s using Quotient.inductionOn
+  induction s using Quotient.ind; rename_i s
   rw [← id_wrap, ← comp_wrap]
   apply Quotient.sound
   intros j
-  rw [Subst'.comp_def]
-  sorry
+  rw [Subst'.comp_def, apply_wrap, id_wrap, id_apply]
 
 @[simp]
 theorem shift_comp_cons : comp (shift σ 1) (cons e s) = s := by
-  induction s using Quotient.inductionOn
+  induction s using Quotient.ind; rename_i s
   rw [← cons_wrap, ← shift_wrap, ← comp_wrap]
   apply Quotient.sound
   intros j
   rw [Subst'.comp_def, Subst'.get, Subst'.apply, Subst'.apply_var]
 
 @[simp]
-theorem cons_comp : comp (cons e s) t = cons (s e) (comp s t) := by
-  induction s using Quotient.inductionOn
-  induction t using Quotient.inductionOn
+theorem cons_comp : comp (cons e s) t = cons (t e) (comp s t) := by
+  induction s using Quotient.ind; rename_i s
+  induction t using Quotient.ind; rename_i t
   simp only [← apply_wrap, ← cons_wrap, ← comp_wrap]
   apply Quotient.sound
   intros j
-  sorry
+  cases j with
+  | zero => rw [Subst'.comp_def, Subst'.get]; rfl
+  | succ j => rw [Subst'.comp_def, Subst'.get, Subst'.get, Subst'.comp_def]
 
 @[simp]
 theorem comp_assoc : comp (comp s t) u = comp s (comp t u) := by
-  induction s using Quotient.inductionOn
-  induction t using Quotient.inductionOn
-  induction u using Quotient.inductionOn
+  induction s using Quotient.ind; rename_i s
+  induction t using Quotient.ind; rename_i t
+  induction u using Quotient.ind; rename_i u
   simp only [← comp_wrap]
   apply Quotient.sound
   intros j
   simp only [Subst'.comp_def, Subst'.apply]
-  sorry
+  simp only [get_wrap, apply_wrap, apply_apply, comp_wrap]
 
 @[simp]
 theorem apply_zero_cons_shift_comp : cons (s (.var 0)) (comp (shift σ 1) s) = s := by
-  induction s using Quotient.inductionOn
-  rw [← shift_wrap, ← apply_wrap, ← comp_wrap, ← cons_wrap]
+  induction s using Quotient.ind; rename_i s
+  rw [← apply_wrap, Subst'.apply_var, ← shift_wrap, ← comp_wrap, ← cons_wrap]
   apply Quotient.sound
   intros j
-  rw [Subst'.apply_var]
-  sorry
+  cases j with
+  | zero => rfl
+  | succ j => rw [Subst'.get, Subst'.comp_def, Subst'.get, Subst'.apply_var]
 
 @[simp]
 theorem zero_cons_shift : cons (.var 0) (shift σ 1) = id σ := by
@@ -258,5 +278,7 @@ theorem zero_cons_shift : cons (.var 0) (shift σ 1) = id σ := by
 example : comp (shift σ 1) (id σ) = shift σ 1 := by
   simp
 -/
+
+end
 
 end Leansubst.Subst
